

# Derivation of $\sigma_{\text{loo,diff}}^2$

## Proofs

The main quantity of interest is the mean expected log pointwise predictive density, which we want to use for model evaluation and comparison.

**Definition 1** ( $\overline{\text{elpd}}$ ). *The mean expected log pointwise predictive density for a model  $p$  is defined as*

$$\overline{\text{elpd}} = \int p_t(x) \log p(x) dx$$

where  $p_t(x) = p(x|\theta_0)$  is the true density at a new unseen observation  $x$  and  $\log p(x)$  is the log predictive density for observation  $x$ .

We estimate  $\overline{\text{elpd}}$  using *leave-one-out cross-validation (loo)*.

**Definition 2** (Leave-one-out cross-validation). *The loo estimator  $\overline{\text{elpd}}_{\text{loo}}$  is given by*

$$\overline{\text{elpd}}_{\text{loo}} = \frac{1}{n} \sum_{i=1}^n \pi_i, \quad (1)$$

where  $\pi_i = \log p(y_i|y_{-i}) = \int \log p(y_i|\theta) p(\theta|y_{-i}) d\theta$ .

To estimate  $\overline{\text{elpd}}_{\text{loo}}$  in turn, we use difference estimator. Definitions follow.

**Definition 3.** *Let  $\tilde{\pi}_i$  be any approximation of  $\pi_i$ . The difference estimator of  $\overline{\text{elpd}}_{\text{loo}}$  based on  $\tilde{\pi}_i$  is given by*

$$\widehat{\overline{\text{elpd}}}_{\text{loo,diff}} = \frac{1}{n} \left( \sum_{i=1}^n \tilde{\pi}_i + \frac{n}{m} \sum_{j \in \mathcal{S}} (\pi_j - \tilde{\pi}_j) \right) = \frac{1}{n} (t_{\tilde{\pi}} + \hat{t}_e),$$

where  $\mathcal{S}$  is the subsample set,  $m$  is the subsampling size, and the probability of subsampling observation  $i$  is  $1/n$ , i.e. the subsample is uniform with replacement.

One important estimator of  $\pi_i$  among others is the importance sampling estimator

$$\log \hat{p}(y_i|y_{-i}) = \log \left( \frac{\frac{1}{S} \sum_{s=1}^S p(y_i|\theta_s) r(\theta_s)}{\frac{1}{S} \sum_{s=1}^S r(\theta_s)} \right), \quad (2)$$

where  $r(\theta)$  is any suitable weight function such that  $0 < r(\theta) < \infty$  for all  $\theta \in \Theta$  and  $(\theta_1, \dots, \theta_S)$  is a sample from a suitable approximation of the posterior  $p(\theta|y)$ . We are in particular interested in the weight function

$$\begin{aligned} r(\theta_s) &= \frac{p(\theta_s|y_{-i}) p(\theta_s|y)}{p(\theta_s|y) q(\theta_s|y)} \\ &\propto \frac{1}{p(y_i|\theta_s)} \frac{p(\theta_s|y)}{q(\theta_s|y)} \end{aligned} \quad (3)$$

and where  $q(\cdot|y)$  is an approximation of the posterior distribution that satisfies for each  $y$  that  $q(\theta|y)$  iff  $\theta \in \Theta$ ,  $\theta_s$  is a sample point from  $q$  and  $S$  is the total posterior sample size. (The condition on  $q$  makes sure that  $0 < r(\theta) < \infty$  for all  $\theta$ .)

In the case of truncated importance sampling, we instead truncate these weights and replace  $r$  with  $r_\tau$  given by

$$r_\tau(\theta_s) = \min(r(\theta_s), \tau), \quad (4)$$

where  $\tau > 0$  is the weight truncation [see Ionides, 2008, for a more elaborate discussion on the choice of  $\tau$ ].

## Proof of Proposition 1

**Proposition 1.** *The estimators  $\widehat{\text{elpd}}_{\text{diff}}$  and  $\hat{\sigma}_{\text{loo}}^2$  are unbiased with regard to  $\text{elpd}_{\text{diff}}$  and  $\sigma_{\text{loo}}^2$ .*

*Proof.* We start out by proving unbiasedness for the general estimator. Write the difference estimator as

$$\widehat{\text{elpd}}_{\text{loo,diff}} = \hat{t}_\pi = \sum_{i=1}^n \tilde{\pi}_i + \frac{n}{m} \sum_{i=1}^n \sum_{j \in \mathcal{S}} I_{ij} (\pi_j - \tilde{\pi}_j),$$

where  $I_{ij}$  is the indicator that data point  $i$  is chosen as the  $j$ 'th point of the subsample. Since  $\mathbb{E}[I_{ij}] = 1/n$ , the expectation of the double sum is  $\sum_i (\pi_i - \tilde{\pi}_i)$  and  $\mathbb{E}[\widehat{\text{elpd}}_{\text{loo,diff}}] = \sum_i \pi_i$  as desired.

Next we prove unbiasedness of  $\hat{\sigma}_{\text{loo,diff}}^2$ . We are interested in estimating the finite sampling variance using the difference estimator. This can be done as

$$\sigma_{\text{loo}}^2 = \frac{1}{n} \sum_{i=1}^n (\pi_i - \bar{\pi})^2 \quad (5)$$

$$= \underbrace{\frac{1}{n} \sum_{i=1}^n \pi_i^2}_a - \underbrace{\left( \frac{1}{n} \sum_{i=1}^n \pi_i \right)^2}_b \quad (6)$$

We can estimate  $a$  and  $b$  separately as follows. The first part can be estimated using the difference estimator with  $\tilde{\pi}_i^2$  as auxiliary variable. Let  $t_\epsilon = \sum_i^n \epsilon_i = \sum_i^n \pi_i^2 - \tilde{\pi}_i^2 = t_{\pi^2} - t_{\tilde{\pi}^2}$ , then we can estimate  $a$  as

$$\hat{a} = \frac{1}{n}(t_{\pi^2} + \hat{t}_\epsilon), \quad (7)$$

where

$$\hat{t}_\epsilon = \frac{n}{m} \sum_{j \in \mathcal{S}} (\pi_j^2 - \tilde{\pi}_j^2).$$

From the previous section, it follows directly that

$$E(\hat{a}) = \frac{1}{n}t_{\pi^2} = \frac{1}{n} \sum_{i=1}^n \pi_i^2,$$

The second part,  $b$ , can then be estimated as

$$\hat{b} = \frac{1}{n^2} [\hat{t}_\epsilon^2 - v(\hat{t}_\epsilon) + 2t_{\tilde{\pi}}\hat{t}_\pi - t_{\tilde{\pi}}^2], \quad (8)$$

with the expectation

$$E(\hat{b}) = \frac{1}{n^2} [E(\hat{t}_\epsilon^2) - E(v(\hat{t}_\epsilon)) + 2t_{\tilde{\pi}}E(\hat{t}_\pi) - t_{\tilde{\pi}}^2] \quad (9)$$

$$= \frac{1}{n^2} [V(\hat{t}_\epsilon) + E(\hat{t}_\epsilon)^2 - V(\hat{t}_\epsilon) + 2t_{\tilde{\pi}}t_\pi - t_{\tilde{\pi}}^2] \quad (10)$$

$$= \frac{1}{n^2} [t_\epsilon^2 + 2t_{\tilde{\pi}}t_\pi - t_{\tilde{\pi}}^2] \quad (11)$$

$$= \frac{1}{n^2} [(t_\pi - t_{\tilde{\pi}})^2 + 2t_{\tilde{\pi}}t_\pi - t_{\tilde{\pi}}^2] \quad (12)$$

$$= \frac{1}{n^2} t_\pi^2 = \left( \frac{1}{n} \sum_i^n \pi_i \right)^2 \quad (13)$$

Using that

$$E(v(\hat{t}_\epsilon)) = n^2 \left(1 - \frac{m}{n}\right) \frac{E(s_e^2)}{m} = n^2 \left(1 - \frac{m}{n}\right) \frac{S_e^2}{m} = V(\hat{t}_\epsilon). \quad (14)$$

Combining the results we have that

$$E(\hat{a} - \hat{b}) = \frac{1}{n} \sum_{i=1}^n \pi_i^2 - \left( \frac{1}{n} \sum_{i=1}^n \pi_i \right)^2 = \sigma_{\text{loo}}^2. \quad (15)$$

□

**Remark.** We believe this has probably been proven before, and hence this is probably not a new theoretical result.

## Derivation of $\sigma_{\text{loo,diff}}^2$

Based on Eq. 6, 7 and 8, we can construct the estimator for  $\sigma_{\text{loo}}^2$  as

$$\sigma_{\text{loo}}^2 = \hat{a} - \hat{b} \quad (16)$$

$$= \underbrace{\frac{1}{n}(t_{\tilde{\pi}^2} + \hat{t}_e)}_{\hat{a}} - \quad (17)$$

$$\underbrace{\frac{1}{n^2} [\hat{t}_e^2 - v(\hat{t}_e) + 2t_{\tilde{\pi}}\hat{t}_\pi - t_{\tilde{\pi}}^2]}_{\hat{b}} \quad (18)$$

$$= \underbrace{\frac{1}{n} \left( \sum_{i=1}^n \tilde{\pi}_i^2 + \frac{n}{m} \sum_{j \in \mathcal{S}} (\pi_j^2 - \tilde{\pi}_j^2) \right)}_{\hat{a}} - \quad (19)$$

$$\underbrace{\frac{1}{n^2} [\hat{t}_e^2 - v(\hat{t}_e)]}_{\hat{b}} - \quad (20)$$

$$\underbrace{\frac{1}{n^2} [2t_{\tilde{\pi}}\hat{t}_\pi - t_{\tilde{\pi}}^2]}_{\hat{b}} \quad (21)$$

$$= \underbrace{\frac{1}{n} \left( \sum_{i=1}^n \tilde{\pi}_i^2 + \frac{n}{m} \sum_{j \in \mathcal{S}} (\pi_j^2 - \tilde{\pi}_j^2) \right)}_{\hat{a}} - \quad (22)$$

$$\underbrace{\frac{1}{n^2} \left[ \left( \frac{n}{m} \sum_{j \in \mathcal{S}} (\pi_j - \tilde{\pi}_j) \right)^2 - v(\hat{t}_\pi) \right]}_{\hat{b}} - \quad (23)$$

$$\underbrace{\frac{1}{n^2} \left[ 2 \left( \sum_{i=1}^n \tilde{\pi}_i \right) \hat{t}_\pi - \left( \sum_{i=1}^n \tilde{\pi}_i \right)^2 \right]}_{\hat{b}} \quad (24)$$

Here, we use that

$$v(\hat{t}_e) = v(\hat{t}_\pi) = V(\widehat{\text{elpd}}_{\text{diff,loo}}),$$

that

$$\hat{t}_\pi = \widehat{\text{elpd}}_{\text{diff,loo}},$$

$$\hat{\sigma}_{\text{diff,loo}}^2 = n\sigma_{\text{loo}}^2 \quad (25)$$

$$= \sum_{i=1}^n \tilde{\pi}_i^2 + \frac{n}{m} \sum_{j \in \mathcal{S}} (\pi_j^2 - \tilde{\pi}_j^2) - \quad (26)$$

$$\frac{1}{n} \left[ \left( \frac{n}{m} \sum_{j \in \mathcal{S}} (\pi_j - \tilde{\pi}_j) \right)^2 - V(\widehat{\text{elpd}}_{\text{diff,loo}}) \right] -$$

$$\frac{1}{n} \left[ 2 \left( \sum_{i=1}^n \tilde{\pi}_i \right) \widehat{\text{elpd}}_{\text{diff,loo}} - \left( \sum_{i=1}^n \tilde{\pi}_i \right)^2 \right].$$

## References

Edward L Ionides. Truncated importance sampling. *Journal of Computational and Graphical Statistics*, 17(2):295–311, 2008.